Formalise semantics down to evalObservation

semantics-3.0/isabelle/Semantics.thy
@@ -14,42 +14,34 @@ type_synonym ChosenNum = int
 
 datatype AccountId = AccountId NumAccount Party
 
-fun less_eq :: "AccountId \<Rightarrow> AccountId \<Rightarrow> bool" where
-"less_eq (AccountId a b) (AccountId c d) =
+(* BEGIN Proof of linorder for AccountId *)
+fun less_eq_AccId :: "AccountId \<Rightarrow> AccountId \<Rightarrow> bool" where
+"less_eq_AccId (AccountId a b) (AccountId c d) =
    (if a < c then True
     else (if (a > c) then False else b \<le> d))"
 
-fun less :: "AccountId \<Rightarrow> AccountId \<Rightarrow> bool" where
-  "less a b = (\<not> (less_eq b a))"
+fun less_AccId :: "AccountId \<Rightarrow> AccountId \<Rightarrow> bool" where
+"less_AccId a b = (\<not> (less_eq_AccId b a))"
 
-(* BEGIN Proof of linorder for AccountId *)
 instantiation "AccountId" :: "ord"
 begin
-definition "a < b = less a b"
-definition "a \<le> b = less_eq a b"
+definition "a \<le> b = less_eq_AccId a b"
+definition "a < b = less_AccId a b"
 instance
 proof
 qed
 end
 
-lemma linearAccountId_aux :
-  "(AccountId x1 x2) \<le> (AccountId y1 y2) \<or>
-   (AccountId y1 y2) \<le> (AccountId x1 x2)"
-  apply (cases "x1 \<le> y1")
-  apply (cases "y1 \<le> y2")
-  by (auto simp: less_eq_AccountId_def linear)
-
 lemma linearAccountId : "x \<le> y \<or> y \<le> (x::AccountId)"
-  by (metis AccountId.exhaust linearAccountId_aux)
-
+  by (smt less_eq_AccId.elims(3) less_eq_AccId.simps less_eq_AccountId_def)
+ 
 instantiation "AccountId" :: linorder
 begin
 instance
 proof
   fix x y
   have "(x < y) = (x \<le> y \<and> \<not> y \<le> (x :: AccountId))"
-    by (meson less.elims(2) less.elims(3) less_AccountId_def
-              less_eq_AccountId_def linearAccountId)
+    by (meson less_AccId.elims(2) less_AccId.elims(3) less_AccountId_def less_eq_AccountId_def linearAccountId)
   thus "(x < y) = (x \<le> y \<and> \<not> y \<le> x)" by simp
 next
   fix x
@@ -58,12 +50,12 @@ next
 next
   fix x y z
   have "x \<le> y \<Longrightarrow> y \<le> z \<Longrightarrow> x \<le> (z :: AccountId)"
-    by (smt less_eq.elims(2) less_eq.simps less_eq_AccountId_def)
+    by (smt less_eq_AccId.elims(2) less_eq_AccId.simps less_eq_AccountId_def)
   thus "x \<le> y \<Longrightarrow> y \<le> z \<Longrightarrow> x \<le> z" by simp
 next
   fix x y z
   have "x \<le> y \<Longrightarrow> y \<le> x \<Longrightarrow> x = (y :: AccountId)"
-    by (smt AccountId.inject less_eq.elims(2) less_eq_AccountId_def)
+    by (smt less_eq_AccId.elims(2) less_eq_AccId.simps less_eq_AccountId_def)
   thus "x \<le> y \<Longrightarrow> y \<le> x \<Longrightarrow> x = (y :: AccountId)" by simp
 next
   fix x y
@@ -77,8 +69,159 @@ fun accountOwner :: "AccountId \<Rightarrow> Party" where
 "accountOwner (AccountId _ party) = party"
 
 datatype ChoiceId = ChoiceId NumChoice Party
+
+(* BEGIN Proof of linorder for ChoiceId *)
+fun less_eq_ChoId :: "ChoiceId \<Rightarrow> ChoiceId \<Rightarrow> bool" where
+"less_eq_ChoId (ChoiceId a b) (ChoiceId c d) =
+   (if a < c then True
+    else (if (a > c) then False else b \<le> d))"
+
+fun less_ChoId :: "ChoiceId \<Rightarrow> ChoiceId \<Rightarrow> bool" where
+"less_ChoId a b = (\<not> (less_eq_ChoId b a))"
+
+instantiation "ChoiceId" :: "ord"
+begin
+definition "a \<le> b = less_eq_ChoId a b"
+definition "a < b = less_ChoId a b"
+instance
+proof
+qed
+end
+
+lemma linearChoiceId : "x \<le> y \<or> y \<le> (x::ChoiceId)"
+  by (smt less_eq_ChoId.elims(3) less_eq_ChoId.simps less_eq_ChoiceId_def)
+ 
+instantiation "ChoiceId" :: linorder
+begin
+instance
+proof
+  fix x y
+  have "(x < y) = (x \<le> y \<and> \<not> y \<le> (x :: ChoiceId))"
+    by (meson less_ChoId.elims(2) less_ChoId.elims(3) less_ChoiceId_def less_eq_ChoiceId_def linearChoiceId)
+  thus "(x < y) = (x \<le> y \<and> \<not> y \<le> x)" by simp
+next
+  fix x
+  have "x \<le> (x :: ChoiceId)" by (meson linearChoiceId)
+  thus "x \<le> x" by simp
+next
+  fix x y z
+  have "x \<le> y \<Longrightarrow> y \<le> z \<Longrightarrow> x \<le> (z :: ChoiceId)"
+    by (smt less_eq_ChoId.elims(2) less_eq_ChoId.simps less_eq_ChoiceId_def)
+  thus "x \<le> y \<Longrightarrow> y \<le> z \<Longrightarrow> x \<le> z" by simp
+next
+  fix x y z
+  have "x \<le> y \<Longrightarrow> y \<le> x \<Longrightarrow> x = (y :: ChoiceId)"
+    by (smt less_eq_ChoId.elims(2) less_eq_ChoId.simps less_eq_ChoiceId_def)
+  thus "x \<le> y \<Longrightarrow> y \<le> x \<Longrightarrow> x = (y :: ChoiceId)" by simp
+next
+  fix x y
+  from linearChoiceId have "x \<le> y \<or> y \<le> (x :: ChoiceId)" by simp
+  thus "x \<le> y \<or> y \<le> x" by simp
+qed
+end
+(* END Proof of linorder for ChoiceId *)
+
 datatype OracleId = OracleId PubKey
+
+(* BEGIN Proof of linorder for OracleId *)
+fun less_eq_OraId :: "OracleId \<Rightarrow> OracleId \<Rightarrow> bool" where
+"less_eq_OraId (OracleId a) (OracleId b) = (a \<le> b)"
+
+fun less_OraId :: "OracleId \<Rightarrow> OracleId \<Rightarrow> bool" where
+"less_OraId (OracleId a) (OracleId b) = (a < b)"
+
+instantiation "OracleId" :: "ord"
+begin
+definition "a \<le> b = less_eq_OraId a b"
+definition "a < b = less_OraId a b"
+instance
+proof
+qed
+end
+
+lemma linearOracleId : "x \<le> y \<or> y \<le> (x::OracleId)"
+  by (smt OracleId.inject less_eq_OraId.elims(3) less_eq_OracleId_def)
+
+instantiation "OracleId" :: linorder
+begin
+instance
+proof
+  fix x y
+  have "(x < y) = (x \<le> y \<and> \<not> y \<le> (x :: OracleId))"
+    by (metis OracleId.exhaust dual_order.order_iff_strict less_OraId.simps less_OracleId_def less_eq_OraId.simps less_eq_OracleId_def not_le)
+  thus "(x < y) = (x \<le> y \<and> \<not> y \<le> x)" by simp
+next
+  fix x
+  have "x \<le> (x :: OracleId)" by (meson linearOracleId)
+  thus "x \<le> x" by simp
+next
+  fix x y z
+  have "x \<le> y \<Longrightarrow> y \<le> z \<Longrightarrow> x \<le> (z :: OracleId)"
+    by (smt OracleId.inject less_eq_OraId.elims(2) less_eq_OraId.elims(3) less_eq_OracleId_def)
+  thus "x \<le> y \<Longrightarrow> y \<le> z \<Longrightarrow> x \<le> z" by simp
+next
+  fix x y z
+  have "x \<le> y \<Longrightarrow> y \<le> x \<Longrightarrow> x = (y :: OracleId)"
+    by (smt less_eq_OraId.elims(2) less_eq_OraId.simps less_eq_OracleId_def)
+  thus "x \<le> y \<Longrightarrow> y \<le> x \<Longrightarrow> x = (y :: OracleId)" by simp
+next
+  fix x y
+  from linearOracleId have "x \<le> y \<or> y \<le> (x :: OracleId)" by simp
+  thus "x \<le> y \<or> y \<le> x" by simp
+qed
+end
+(* END Proof of linorder for OracleId *)
+
 datatype ValueId = ValueId int
+
+(* BEGIN Proof of linorder for ValueId *)
+fun less_eq_ValId :: "ValueId \<Rightarrow> ValueId \<Rightarrow> bool" where
+"less_eq_ValId (ValueId a) (ValueId b) = (a \<le> b)"
+
+fun less_ValId :: "ValueId \<Rightarrow> ValueId \<Rightarrow> bool" where
+"less_ValId (ValueId a) (ValueId b) = (a < b)"
+
+instantiation "ValueId" :: "ord"
+begin
+definition "a \<le> b = less_eq_ValId a b"
+definition "a < b = less_ValId a b"
+instance
+proof
+qed
+end
+
+lemma linearValueId : "x \<le> y \<or> y \<le> (x::ValueId)"
+  by (smt ValueId.inject less_eq_ValId.elims(3) less_eq_ValueId_def)
+
+instantiation "ValueId" :: linorder
+begin
+instance
+proof
+  fix x y
+  have "(x < y) = (x \<le> y \<and> \<not> y \<le> (x :: ValueId))"
+    by (metis ValueId.exhaust dual_order.order_iff_strict less_ValId.simps less_ValueId_def less_eq_ValId.simps less_eq_ValueId_def not_le)
+  thus "(x < y) = (x \<le> y \<and> \<not> y \<le> x)" by simp
+next
+  fix x
+  have "x \<le> (x :: ValueId)" by (meson linearValueId)
+  thus "x \<le> x" by simp
+next
+  fix x y z
+  have "x \<le> y \<Longrightarrow> y \<le> z \<Longrightarrow> x \<le> (z :: ValueId)"
+    by (smt ValueId.inject less_eq_ValId.elims(2) less_eq_ValId.elims(3) less_eq_ValueId_def)
+  thus "x \<le> y \<Longrightarrow> y \<le> z \<Longrightarrow> x \<le> z" by simp
+next
+  fix x y z
+  have "x \<le> y \<Longrightarrow> y \<le> x \<Longrightarrow> x = (y :: ValueId)"
+    by (smt less_eq_ValId.elims(2) less_eq_ValId.simps less_eq_ValueId_def)
+  thus "x \<le> y \<Longrightarrow> y \<le> x \<Longrightarrow> x = (y :: ValueId)" by simp
+next
+  fix x y
+  from linearValueId have "x \<le> y \<or> y \<le> (x :: ValueId)" by simp
+  thus "x \<le> y \<or> y \<le> x" by simp
+qed
+end
+(* END Proof of linorder for ValueId *)
 
 datatype Value = AvailableMoney AccountId
                | Constant int
@@ -151,5 +294,62 @@ fun addOutcome :: "Party \<Rightarrow> Money \<Rightarrow> TransactionOutcomes \
 
 fun combineOutcomes :: "TransactionOutcomes \<Rightarrow> TransactionOutcomes \<Rightarrow> TransactionOutcomes" where
 "combineOutcomes x y = MList.unionWith plus x y"
+
+datatype IntervalError = InvalidInterval SlotInterval
+                       | IntervalInPastError SlotNumber SlotInterval
+
+datatype IntervalResult = IntervalTrimmed Environment State
+                        | IntervalError IntervalError
+
+fun fixInterval :: "SlotInterval \<Rightarrow> State \<Rightarrow> IntervalResult" where
+"fixInterval (l, h) st =
+   (let minSlot = minSlot st in
+    let nl = max l minSlot in
+    let tInt = (nl, h) in
+    let env = \<lparr> slotInterval = tInt \<rparr> in
+    let nst = st \<lparr> minSlot := nl \<rparr> in
+    (if (h < l)
+     then IntervalError (InvalidInterval (l, h))
+     else (if (h < minSlot)
+           then IntervalError (IntervalInPastError minSlot (l, h))
+           else IntervalTrimmed env nst)))"
+
+fun evalValue :: "Environment \<Rightarrow> State \<Rightarrow> Value \<Rightarrow> int" where
+"evalValue env state (AvailableMoney accId) =
+    findWithDefault 0 accId (account state)" |
+"evalValue env state (Constant integer) = integer" |
+"evalValue env state (NegValue val) = evalValue env state val" |
+"evalValue env state (AddValue lhs rhs) =
+    evalValue env state lhs + evalValue env state rhs" |
+"evalValue env state (SubValue lhs rhs) =
+    evalValue env state lhs + evalValue env state rhs" |
+"evalValue env state (ChoiceValue choId defVal) =
+    findWithDefault (evalValue env state defVal) choId (choice state)" |
+"evalValue env state (SlotIntervalStart) = fst (slotInterval env)" |
+"evalValue env state (SlotIntervalEnd) = snd (slotInterval env)" |
+"evalValue env state (UseValue valId) =
+    findWithDefault 0 valId (boundValues state)"
+
+fun evalObservation :: "Environment \<Rightarrow> State \<Rightarrow> Observation \<Rightarrow> bool" where
+"evalObservation env state (AndObs lhs rhs) =
+    (evalObservation env state lhs \<and> evalObservation env state rhs)" |
+"evalObservation env state (OrObs lhs rhs) =
+    (evalObservation env state lhs \<or> evalObservation env state rhs)" |
+"evalObservation env state (NotObs subObs) =
+    (\<not> evalObservation env state subObs)" |
+"evalObservation env state (ChoseSomething choId) =
+    (member choId (choice state))" |
+"evalObservation env state (ValueGE lhs rhs) =
+    (evalValue env state lhs \<ge> evalValue env state rhs)" |
+"evalObservation env state (ValueGT lhs rhs) =
+    (evalValue env state lhs > evalValue env state rhs)" |
+"evalObservation env state (ValueLT lhs rhs) =
+    (evalValue env state lhs < evalValue env state rhs)" |
+"evalObservation env state (ValueLE lhs rhs) =
+    (evalValue env state lhs \<le> evalValue env state rhs)" |
+"evalObservation env state (ValueEQ lhs rhs) =
+    (evalValue env state lhs = evalValue env state rhs)" |
+"evalObservation env state TrueObs = True" |
+"evalObservation env state FalseObs = False"
 
 end
